Soundness.v
@@ -10,21 +10,42 @@ Require Import ConcreteInterpreter.
 Require Import Galois.
 Require Import Language.
 Require Import Maps.
+Require Import Monad.
 Require Import Parity.
 Require Import Preorder.
-Open Scope com_scope.
 
 Definition sound {A B A' B' : Type} 
-  `{Galois A B} `{Galois A' B'}
-  (f : A->A') (f' : B->B') :=
-  forall b a, gamma b a -> gamma (f' b) (f a).
+  `{Galois B A} `{Galois B' A'}
+  (f : B->B') (f' : A->A') :=
+  forall b a, gamma a b -> gamma (f' a) (f b).
+  
+Lemma bind_state_sound {S S' A A' B B'} 
+`{Galois S S', Galois A A', Galois B B'}
+: 
+forall next next' f f',
+sound f f' ->
+sound next next' ->
+sound (bind_state S A B f next) (bind_state S' A' B' f' next').
+Proof.
+  intros. simpl. unfold gamma_fun. intros. simpl. unfold sound. intros b a H10.
+  simpl. unfold bind_state. unfold sound in H8. 
+  assert (gamma (f' a) (f b)); auto. 
+  destruct (f' a) eqn:Hf'a; destruct (f b) eqn:Hfb.
+  - destruct p, p0. apply H9. simpl in H11. apply H11. apply H11.
+  - inversion H11.
+  - simpl.  destruct p. destruct (next a0 s); reflexivity.
+  - reflexivity. 
+Qed.
 
+Tactic Notation "bind" := apply bind_state_sound;[auto| |auto].
+
+Tactic Notation "pairs" := unfold gamma_pairs; simpl; split.
 
 Lemma sound_parity_plus :
-  (gamma parity_plus) plus.
+  sound plus parity_plus.
 Proof. intros ? ? ? ? ? ?.
   unfold sound. simpl. unfold gamma_fun; intros. simpl. 
-  destruct b, b0; simpl in *; try tauto;
+  destruct a, a0; simpl in *; try tauto;
   auto using even_even_plus, odd_plus_r, odd_plus_l, odd_even_plus.
 Qed.
 
@@ -32,7 +53,7 @@ Lemma sound_parity_mult :
   sound mult parity_mult.
 Proof. 
   unfold sound. simpl. unfold gamma_fun. intros. simpl.
-  destruct b, b0; simpl in *; try tauto; 
+  destruct a, a0; simpl in *; try tauto; 
   auto using even_mult_l, even_mult_r, odd_mult.
 Qed.
 
@@ -40,7 +61,7 @@ Lemma sound_parity_eq :
   sound Nat.eqb parity_eq.
 Proof.
   unfold sound. simpl. unfold gamma_fun. intros.
-  destruct b, b0; simpl in *; try tauto; unfold not; intros.
+  destruct a, a0; simpl in *; try tauto; unfold not; intros.
   - apply Bool.Is_true_eq_true in H1. apply Nat.eqb_eq in H1. subst.
     eauto using not_even_and_odd. 
   - apply Bool.Is_true_eq_true in H1. apply Nat.eqb_eq in H1. subst.
@@ -68,3 +89,181 @@ Proof.
   destruct b, a; simpl in *; tauto.
 Qed.
 
+Theorem eval_aexp_sound :
+  forall a, sound (eval_aexp a) (abstract_eval_aexp a).
+Proof.
+  intros.
+  unfold sound. simpl.
+  induction a.
+  - (* ANum *) simpl. unfold gamma_pairs; simpl. split.
+    + apply gamma_par_extract_n_n.
+    + apply H.
+  - (* AVar *) simpl. unfold gamma_pairs; simpl. split.
+    + simpl in H. unfold gamma_store in H. apply H.
+    + apply H.
+  - (* APlus *) simpl in *. intros st ast H. apply bind_state_sound.
+    + unfold sound. intros st' ast' Hgamma. simpl in Hgamma. 
+      apply IHa1. apply Hgamma.
+    + unfold sound. intros n p Hgamma. simpl. unfold gamma_fun. 
+      intros ast' st'. intros Hstore. simpl. apply bind_state_sound.
+      * unfold sound. intros st'' ast''. intros Hgamma'. apply IHa2.
+        assumption.
+      * unfold sound. intros n' p' Hgamma'. simpl. unfold gamma_fun.
+        intros ast'' st'' Hgamma''. simpl. unfold gamma_pairs; simpl; split.
+        { apply sound_parity_plus; assumption. }
+        { apply Hgamma''. }
+      * apply Hstore.
+    + apply H.
+  - (* AMult *) intros st ast Hstore. simpl. 
+    apply bind_state_sound; unfold sound.
+    + intros st' ast' Hstore'. simpl. apply IHa1; assumption.
+    + intros n p Hpar. simpl. unfold gamma_fun. intros ast' st' Hstore'.
+      simpl. apply bind_state_sound.
+      * unfold sound. intros st'' ast'' Hstore''. simpl. apply IHa2. 
+        apply Hstore''.
+      * unfold sound. intros n' p' Hpar'. simpl. unfold gamma_fun.
+        intros ast'' st'' Hstore''. simpl. unfold gamma_pairs;simpl;split.
+        { apply sound_parity_mult; assumption. }
+        { apply Hstore''. }
+      * apply Hstore'.
+    + apply Hstore.
+Qed.
+
+Lemma eval_bexp_beq_sound : forall n n',
+sound (eval_aexp n) (abstract_eval_aexp n) ->
+sound (eval_aexp n') (abstract_eval_aexp n') ->
+sound (eval_bexp (BEq n n')) (beval_abstract (BEq n n')).
+Proof. 
+  unfold sound. simpl. intros a a' IH1 IH2 st ast Hstore. simpl. 
+  bind.
+  unfold sound. intros n p Hpar. simpl. unfold gamma_fun.
+  intros ast' st' Hstore'. simpl. bind. 
+  unfold sound. intros n' p' Hpar'. simpl. unfold gamma_fun.
+  intros ast'' st'' Hstore''. simpl. unfold gamma_pairs;simpl;split.
+  apply sound_parity_eq. assumption. assumption. assumption.
+Qed.
+
+Lemma eval_bexp_ble_sound : forall n n', 
+sound (eval_aexp n) (abstract_eval_aexp n) ->
+sound (eval_aexp n') (abstract_eval_aexp n') ->
+sound (eval_bexp (BLe n n')) (beval_abstract (BLe n n')).
+Proof. 
+  intros a a' H1 H2. simpl. apply bind_state_sound. assumption.
+  unfold sound. intros n p Hpar. simpl. unfold gamma_fun. intros ast st Hstore.
+  simpl. bind. unfold sound. intros n' p' Hpar'. simpl. unfold gamma_fun. 
+  intros ast' st' Hstore'. simpl. pairs; auto.
+Qed.
+
+Lemma eval_bexp_not_sound : forall b,
+sound (eval_bexp b) (beval_abstract b) ->
+sound (eval_bexp (BNot b)) (beval_abstract (BNot b)).
+Proof. 
+  intros b H.
+  unfold sound. intros st ast Hstore. simpl. bind.
+  unfold sound. intros b' ab Hbool. simpl. unfold gamma_fun. 
+    intros aast' st' Hstore'. pairs.
+    + apply sound_ab_neg. apply Hbool.
+    + apply Hstore'.
+Qed.
+
+Lemma eval_bexp_and_sound : forall b1 b2,
+sound (eval_bexp b1) (beval_abstract b1) ->
+sound (eval_bexp b2) (beval_abstract b2) ->
+sound (eval_bexp (BAnd b1 b2)) (beval_abstract (BAnd b1 b2)).
+Proof. 
+  intros b1 b2 H1 H2. unfold sound. intros st ast Hstore.
+  simpl. bind. unfold sound. intros b ab Hbool. simpl. unfold gamma_fun.
+    intros ast' st' Hstore'. simpl. bind.
+    + unfold sound. intros b' ab' Hbool'. simpl. unfold gamma_fun.
+      intros ast'' st'' Hstore''. simpl. pairs.
+      * apply sound_ab_and; assumption.
+      * assumption.
+Qed.
+
+Theorem eval_bexp_sound :
+  forall b, sound (eval_bexp b) (beval_abstract b).
+Proof.
+  induction b.
+  - simpl. unfold sound. intros st ast Hstore. simpl. 
+    unfold gamma_pairs; simpl; split; auto.
+  - simpl. unfold sound. intros st ast Hstore. simpl.
+    unfold gamma_pairs; simpl; split; auto.
+  - apply eval_bexp_beq_sound; apply eval_aexp_sound.
+  - apply eval_bexp_ble_sound; apply eval_aexp_sound.
+  - apply eval_bexp_not_sound. apply IHb.
+  - apply eval_bexp_and_sound; assumption.
+Qed.
+
+Lemma sound_seq : forall c1 c2,
+  sound (ceval c1) (ceval_abstract c1) ->
+  sound (ceval c2) (ceval_abstract c2) ->
+  sound (ceval (c1 ;c; c2)) (ceval_abstract (c1 ;c; c2)).
+Proof.
+  intros c1 c2 H1 H2. unfold sound. intros. simpl. bind.
+  unfold sound. intros. simpl. unfold gamma_fun. intros.
+    unfold sound in H2. apply H2. apply H3.
+Qed.
+
+Lemma sound_assignment : forall x a,
+  sound (ceval (CAss x a)) (ceval_abstract (CAss x a)).
+Proof. 
+  intros. unfold sound. intros. bind.
+  - apply eval_aexp_sound.
+  - simpl. unfold sound. intros. simpl. unfold gamma_fun. intros.
+    simpl. unfold gamma_pairs. simpl. split.
+    + constructor.
+    + unfold gamma_store. intros x'. apply t_update_sound; assumption.
+Qed.
+  
+Lemma sound_if : forall b c1 c2,
+  sound (ceval c1) (ceval_abstract c1) ->
+  sound (ceval c2) (ceval_abstract c2) ->
+  sound (ceval (CIf b c1 c2)) (ceval_abstract (CIf b c1 c2)).
+Proof. 
+  intros. simpl. apply bind_state_sound. 
+  - apply eval_bexp_sound.
+  - unfold sound. intros. simpl. unfold gamma_fun. intros. simpl.
+    unfold eval_if_abstract. unfold eval_if. destruct a.
+    + destruct b0. apply H. apply H2. inversion H1.
+    + destruct b0. 
+      * simpl in *. unfold not in H1. exfalso. apply H1. reflexivity.
+      * apply H0. apply H2.
+    + admit. 
+    + inversion H1.
+Admitted.
+
+Lemma sound_try_catch : forall c1 c2,
+  sound (ceval c1) (ceval_abstract c1) ->
+  sound (ceval c2) (ceval_abstract c2) ->
+  sound (ceval (CTryCatch c1 c2)) (ceval_abstract (CTryCatch c1 c2)).
+Proof.
+  intros c1 c2 H1 H2. simpl. unfold sound. intros st ast Hstore.
+  simpl. unfold eval_catch. destruct (ceval_abstract c1 ast) eqn:Habs1.
+  - destruct (ceval c1 st) eqn:Hconc1. 
+    + rewrite <- Habs1, <- Hconc1. unfold sound in H1. apply H1. assumption.
+    + unfold sound in H1. simpl in H1. 
+      assert (gamma_option (ceval_abstract c1 ast) (ceval c1 st)).
+      { apply H1. apply Hstore. }
+      rewrite Habs1 in H. rewrite Hconc1 in H. inversion H.
+  - destruct (ceval c1 st) eqn:Hconc1. 
+    + unfold sound in H1. simpl in *. 
+      destruct (ceval_abstract c2 ast).
+      * simpl. destruct p, p0. pairs.
+        { reflexivity. }
+        { admit. }
+      * reflexivity.
+    + apply H2. apply Hstore.
+Admitted.
+
+Theorem sound_interpreter:
+  forall c, sound (ceval c) (ceval_abstract c).
+Proof.
+  intros. induction c; unfold sound; intros.
+  - (* SKIP *) simpl in *. unfold gamma_pairs. simpl.
+    split; auto; reflexivity.
+  - (* Sequence *) apply sound_seq; assumption.
+  - (* Assignment *) apply sound_assignment; assumption.
+  - (* If *) apply sound_if; assumption.
+  - (* Try-Catch *) apply sound_try_catch; assumption.
+  - (* Fail *) reflexivity.
+Qed.
